WIP: repaired whole compilation, before changing the mem type

backend/Inliningproof.v
@@ -449,13 +449,11 @@ Qed.
 
 
 (** ** Relating stacks *)
-Definition injw_sup_l w := Mem.support (injw_mem_l w).
-Definition injw_sup_r w := Mem.support (injw_mem_r w).
 
 Inductive match_stacks (F: meminj) (m m': mem):
              list stackframe -> list stackframe -> sup -> Prop :=
   | match_stacks_nil: forall support
-        (MG: inj_incr w (injw F m m'))
+        (MG: inj_incr w (injw F (Mem.support m) (Mem.support m')))
         (BELOW: Mem.sup_include (injw_sup_r w) support),
       match_stacks F m m' nil nil support
   | match_stacks_cons: forall res f sp pc rs stk f' sp' sps' rs' stk' support fenv ctx
@@ -543,23 +541,21 @@ Variable F1: meminj.
 Variables m1 m1': mem.
 Hypothesis INCR: inject_incr F F1.
 
-Lemma mit_incr_invariant bound m0 m2 m0' m2':
+Lemma mit_incr_invariant bound s1 s2 s1' s2':
   (forall b1 b2 delta, F1 b1 = Some(b2, delta) -> sup_In b1 (injw_sup_l w) \/ sup_In b2 bound ->
                        F b1 = Some(b2, delta)) ->
-  Mem.sup_include (Mem.support (injw_mem_r w)) bound ->
-  inj_incr w (injw F m0 m2) ->
-  Mem.sup_include (Mem.support m0) (Mem.support m0') ->
-  Mem.sup_include (Mem.support m2) (Mem.support m2') ->
-  max_perm_decrease m0 m0' ->
-  max_perm_decrease m2 m2' ->
-  inj_incr w (injw F1 m0' m2').
+  Mem.sup_include (injw_sup_r w) bound ->
+  inj_incr w (injw F s1 s2) ->
+  Mem.sup_include s1 s1' ->
+  Mem.sup_include s2 s2' ->
+  inj_incr w (injw F1 s1' s2').
 Proof.
   intros INJ BELOW H Hs1' Hs2'. inv H. split; cbn in *; eauto; try extlia.
   eapply inject_incr_trans; eauto.
   intros b1 b2 delta Hb1 Hb1'.
   destruct (F b1) as [[xb1' xdelta]|] eqn:Hb1''.
   - rewrite (INCR _ _ _ Hb1'') in Hb1'. inv Hb1'. eauto.
-  - destruct (Mem.sup_dec b1 (Mem.support m3)); try (erewrite INJ in Hb1''; eauto; discriminate).
+  - destruct (Mem.sup_dec b1 s0); try (erewrite INJ in Hb1''; eauto; discriminate).
     destruct (Mem.sup_dec b2 bound); try (erewrite INJ in Hb1''; eauto; discriminate).
     split; eauto.
 Qed.
@@ -567,11 +563,9 @@ Qed.
 Lemma match_stacks_invariant:
   forall stk stk' support, match_stacks F m m' stk stk' support ->
   forall (INJ: forall b1 b2 delta, F1 b1 = Some(b2, delta) ->
-               sup_In b1 (Mem.support (injw_mem_l w)) \/ sup_In b2 support -> F b1 = Some(b2, delta))
+               sup_In b1 (injw_sup_l w) \/ sup_In b2 support -> F b1 = Some(b2, delta))
          (NB: Mem.sup_include (Mem.support m) (Mem.support m1))
          (TNB: Mem.sup_include (Mem.support m') (Mem.support m1'))
-         (PERMD1 : max_perm_decrease m m1)
-         (PERMD2 : max_perm_decrease m' m1')
          (PERM1: forall b1 b2 delta ofs,
                F1 b1 = Some(b2, delta) -> sup_In b2 support ->
                Mem.perm m1 b1 ofs Max Nonempty -> Mem.perm m b1 ofs Max Nonempty)
@@ -591,9 +585,9 @@ with match_stacks_inside_invariant:
          (TNB: Mem.sup_include (Mem.support m') (Mem.support m1'))
          (INJ: forall b1 b2 delta,
                F1 b1 = Some(b2, delta) ->
-               sup_In b1 (Mem.support (injw_mem_l w)) \/ sup_In b2 (sup_incr sps') -> F b1 = Some(b2, delta))
-         (PERMD1 : max_perm_decrease m m1)
-         (PERMD2 : max_perm_decrease m' m1')
+               sup_In b1 (injw_sup_l w) \/ sup_In b2 (sup_incr sps') -> F b1 = Some(b2, delta))
+(*         (PERMD1 : max_perm_decrease m m1)
+         (PERMD2 : max_perm_decrease m' m1') *)
          (PERM1: forall b1 b2 delta ofs,
                F1 b1 = Some(b2, delta) -> sup_In b2 (sup_incr sps') ->
                Mem.perm m1 b1 ofs Max Nonempty -> Mem.perm m b1 ofs Max Nonempty)
@@ -716,8 +710,10 @@ Proof.
   eapply match_stacks_inside_invariant; eauto with mem.
   rewrite (Mem.support_store _ _ _ _ _ _ H0). eauto.
   rewrite (Mem.support_store _ _ _ _ _ _ H1). eauto.
+(*
+  TODO: legacy proof of MAXPERMDECREASE in internel steps: REMOVE OR USE THEM
   red. intros. eapply Mem.perm_store_2; eauto.
-  red. intros. eapply Mem.perm_store_2; eauto.
+  red. intros. eapply Mem.perm_store_2; eauto. *)
 Qed.
 
 (** Preservation by an allocation *)
@@ -772,7 +768,7 @@ Proof.
   intros. eapply match_stacks_invariant; eauto.
   rewrite (Mem.support_free _ _ _ _ _ H0). eauto.
   red. intros. eapply Mem.perm_free_3; eauto.
-  intros. eapply Mem.perm_free_3; eauto.
+(*  intros. eapply Mem.perm_free_3; eauto. *)
 Qed.
 
 Lemma match_stacks_free_right:
@@ -784,7 +780,7 @@ Lemma match_stacks_free_right:
 Proof.
   intros. eapply match_stacks_invariant; eauto.
   rewrite (Mem.support_free _ _ _ _ _ H1). eauto.
-  red. intros. eapply Mem.perm_free_3; eauto.
+(*  red. intros. eapply Mem.perm_free_3; eauto. *)
   intros. eapply Mem.perm_free_1; eauto with ordered_type.
   left.  subst sp. intro. subst b. eapply freshness; eauto.
   intros. eapply Mem.perm_free_3; eauto.
@@ -1093,8 +1089,10 @@ Proof.
   eapply match_stacks_invariant; eauto.
     rewrite (Mem.support_free _ _ _ _ _ H2). eauto.
     rewrite (Mem.support_free _ _ _ _ _ FREE). eauto.
+(*
     red. intros. eapply Mem.perm_free_3; eauto.
     red. intros. eapply Mem.perm_free_3; eauto.
+*)
     intros. eapply Mem.perm_free_3; eauto.
     intros. eapply Mem.perm_free_1; eauto with ordered_type.
     intros. left. intro. subst b. eapply freshness; eauto.
@@ -1115,7 +1113,7 @@ Proof.
   eapply match_stacks_untailcall; eauto.
   eapply match_stacks_inside_invariant; eauto.
     rewrite (Mem.support_free _ _ _ _ _ H2). eauto.
-    red. intros. eapply Mem.perm_free_3; eauto.
+    (* red. intros. eapply Mem.perm_free_3; eauto. *)
     intros. eapply Mem.perm_free_3; eauto.
   eapply ros_address_agree; eauto.
   eapply agree_val_regs; eauto.
@@ -1128,7 +1126,7 @@ Proof.
   eapply match_stacks_inside_inlined_tailcall; eauto.
   eapply match_stacks_inside_invariant; eauto.
     rewrite (Mem.support_free _ _ _ _ _ H2). eauto.
-    red. intros. eapply Mem.perm_free_3; eauto.
+    (* red. intros. eapply Mem.perm_free_3; eauto. *)
     intros. eapply Mem.perm_free_3; eauto.
   apply agree_val_regs_gen; auto.
   eapply Mem.free_left_inject; eauto.
@@ -1195,8 +1193,9 @@ Proof.
   eapply match_stacks_invariant; eauto.
     rewrite (Mem.support_free _ _ _ _ _ H0). eauto.
     rewrite (Mem.support_free _ _ _ _ _ FREE). eauto.
+(*    red. intros. eapply Mem.perm_free_3; eauto. 
     red. intros. eapply Mem.perm_free_3; eauto.
-    red. intros. eapply Mem.perm_free_3; eauto.
+*)
     intros. eapply Mem.perm_free_3; eauto.
     intros. eapply Mem.perm_free_1; eauto with ordered_type.
     intros. left. intro. subst b. eapply freshness; eauto.
@@ -1217,7 +1216,7 @@ Proof.
   econstructor; eauto.
   eapply match_stacks_inside_invariant; eauto.
     rewrite (Mem.support_free _ _ _ _ _ H0). eauto.
-    red. intros. eapply Mem.perm_free_3; eauto.
+(*    red. intros. eapply Mem.perm_free_3; eauto. *)
     intros. eapply Mem.perm_free_3; eauto.
   destruct or; simpl. apply agree_val_reg; auto. auto.
   eapply Mem.free_left_inject; eauto.
